eliminated need for `Seq.Find.find_lemma`.

src/spec/Flutterbye.Seq.Find.fst
@@ -38,11 +38,11 @@ private type found_p (#a_t:Type) (f:(a_t -> Tot bool)) (s:seq a_t) (i:option nat
             x < get i ==> not (f (index s x))))))
 
 private val find_loop:
-   f:('a -> Tot bool) -> 
-   s:seq 'a -> 
-   i:nat{i <= length s} -> 
-   ac:(option nat) -> 
-   Tot (option nat)
+      f:('a -> Tot bool)
+   -> s:seq 'a
+   -> i:nat{i <= length s}
+   -> ac:(option nat){found_p f (slice s 0 i) ac}
+   -> Tot (ac':option nat{found_p f s ac'})
       (decreases (length s - i))
 let rec find_loop f s i ac =
    if i < length s then
@@ -55,30 +55,9 @@ let rec find_loop f s i ac =
    else
       ac
 
-private val find_lemma:
-   f:('a -> Tot bool) -> 
-   s:seq 'a -> 
-   i:nat{i <= length s} -> 
-   ac:(option nat) -> 
-   Lemma
-      (requires (found_p f (slice s 0 i) ac))
-      (ensures (found_p f s (find_loop f s i ac)))
-      (decreases (length s - i))
-let rec find_lemma f s i ac =
-   if i < length s then
-      let ac' =
-         if is_None ac && f (index s i) then
-            Some i
-         else
-            ac in
-      find_lemma f s (i + 1) ac'
-   else
-      ()
-
 val find: 
    f:('a -> Tot bool) -> 
    s:seq 'a -> 
    Tot (i:option nat{found_p f s i})
 let find f s =
-   find_lemma f s 0 None;
    find_loop f s 0 None
